Add context syntax

Stlc/Typing.lean
@@ -12,7 +12,6 @@ instance : EmptyCollection Context :=
 def Context.update (Γ : Context) (x : String) (τ : Ty) : Context :=
   Function.update Γ x (some τ)
 
-notation:arg x " ↦ " τ "; " Γ:arg => Context.update Γ x τ
 
 def Context.IncludedIn (Γ Γ' : Context) : Prop :=
   ∀ ⦃x τ⦄, Γ x = some τ → Γ' x = some τ
@@ -24,7 +23,7 @@ theorem Context.includedIn_empty (Γ : Context) : ∅ ⊆ Γ := by
   rintro _ _ ⟨⟩
 
 theorem Context.includedIn_update {Γ Γ' : Context} {x : String} {τ : Ty} :
-    Γ ⊆ Γ' → x ↦ τ; Γ ⊆ x ↦ τ; Γ' := by
+    Γ ⊆ Γ' → Γ.update x τ ⊆ Γ'.update x τ := by
   simp only [Subset, IncludedIn, update, Function.update_apply]
   intro h₁ y τ' h₂
   rw [←h₂]
@@ -51,19 +50,34 @@ theorem Context.update_comm {x₁ x₂ : String} (h : x₁ ≠ x₂) (τ₁ τ�
     (Γ.update x₁ τ₁).update x₂ τ₂ = (Γ.update x₂ τ₂).update x₁ τ₁ := by
   exact Function.update_comm h τ₁ τ₂ Γ
 
+namespace Syntax
+
+declare_syntax_cat stlc_ctx
+scoped syntax stlc_ident : stlc_ctx
+scoped syntax "∅" : stlc_ctx
+scoped syntax stlc_ctx "; " term:arg " ↦ " term:arg : stlc_ctx
+scoped syntax "Γ[ " stlc_ctx " ]" : term
+
+scoped macro_rules
+| `(Γ[ $x:stlc_ident ]) => `(x[$x])
+| `(Γ[ ∅ ]) => `((∅ : Context))
+| `(Γ[ $Γ:stlc_ctx; $x:term ↦ $τ:term ]) => `(Context.update Γ[$Γ] $x $τ)
+
+end Syntax
+
 section
 set_option hygiene false
 
 open Syntax
 
-local syntax term " ⊢ " stlc_term " : " stlc_ty : term
+local syntax stlc_ctx " ⊢ " stlc_term " : " stlc_ty : term
 
 local macro_rules
-| `($Γ:term ⊢ $t:stlc_term : $τ:stlc_ty) => `(Judgement $Γ t[$t] τ[$τ])
+| `($Γ:stlc_ctx ⊢ $t:stlc_term : $τ:stlc_ty) => `(Judgement Γ[$Γ] t[$t] τ[$τ])
 
 inductive Judgement : Context → Term → Ty → Prop
 | var {Γ x τ} : Γ x = some τ → Γ ⊢ xⱽ : τ
-| abs {Γ x τ₁ τ₂ t} : (x ↦ τ₂; Γ ⊢ t : τ₁) → Γ ⊢ λ x : τ₂, t : τ₂ → τ₁
+| abs {Γ x τ₁ τ₂ t} : (Γ; x ↦ τ₂ ⊢ t : τ₁) → Γ ⊢ λ x : τ₂, t : τ₂ → τ₁
 | app {Γ τ τ' t₁ t₂} : (Γ ⊢ t₁ : τ → τ') → (Γ ⊢ t₂ : τ) → Γ ⊢ t₁ t₂ : τ'
 | bool {Γ} b : Γ ⊢ $(.bool b) : Bool
 | ite {Γ τ t₁ t₂ t₃} : (Γ ⊢ t₁ : Bool) → (Γ ⊢ t₂ : τ) → (Γ ⊢ t₃ : τ) → Γ ⊢ if t₁ then t₂ else t₃ : τ
@@ -75,12 +89,12 @@ notation Γ " ⊢ " t " : " τ => Judgement Γ t τ
 
 namespace Syntax
 
-scoped syntax term " ⊢' " stlc_term " : " stlc_ty : term
+scoped syntax stlc_ctx " ⊢' " stlc_term " : " stlc_ty : term
 scoped syntax "⊢' " stlc_term " : " stlc_ty : term
 
 scoped macro_rules
-| `($Γ:term ⊢' $t:stlc_term : $τ:stlc_ty) => `(Judgement $Γ t[$t] τ[$τ])
-| `(⊢' $t:stlc_term : $τ:stlc_ty) => `(Judgement ∅ t[$t] τ[$τ])
+| `($Γ:stlc_ctx ⊢' $t:stlc_term : $τ:stlc_ty) => `(Γ[$Γ] ⊢ t[$t] : τ[$τ])
+| `(⊢' $t:stlc_term : $τ:stlc_ty) => `(∅ ⊢ t[$t] : τ[$τ])
 
 end Syntax
 
